theorems: basic AC for addition

theorems/iN/iN_def.lean
@@ -19,122 +19,205 @@ abbrev i128 := iN 128
 instance : OfNat (iN n) val where
   ofNat := iN.bitvec (BitVec.ofNat n val)
 
-/--
-Pick a value for poison. If `x` is poison, return `value`. Otherwise return `x`.
+instance : Coe Bool (iN 1) where
+  coe b := bif b then iN.bitvec 1 else iN.bitvec 0
 
-LangRef: https://llvm.org/docs/LangRef.html#poison-values
--/
-def iN.liftPoison {n} (x value : iN n) : iN n :=
-  match x with
-  | poison => value
-  | _ => x
+instance : Coe (BitVec n) (iN n) where
+  coe b := iN.bitvec b
 
-/- /-- Theorem for normalising the iN literal representation. -/
 @[simp]
-theorem iN.ofNat_eq_bitvec {n : PNat} (val : Nat) :
-  ((no_index OfNat.ofNat val) : iN n) = bitvec (no_index OfNat.ofNat val) := rfl -/
+theorem ofNat_eq_bitvec_ofNat {n val} :
+  (no_index (OfNat.ofNat val) : iN n) = iN.bitvec (BitVec.ofNat n val) := rfl
 
 /-- Macro for matching iN literals in simp-theorems. The normal form that is matched is `iN.ofNat_eq_bitvec`. -/
 macro "lit(" val:term ")" : term => `(no_index bitvec (BitVec.ofNat _ $val))
 
-/- macro "ofNat(" n:term ")" : term => `(no_index (OfNat.ofNat $n))
+protected def iN.poisonWrapper {n} {k} (g : BitVec n → BitVec n → iN k) : iN n → iN n → iN k
+  | poison, _ => poison
+  | _, poison => poison
+  | bitvec a, bitvec b => g a b
 
- -/
+protected def iN.poisonPreconditions {n}
+    (isPoison : BitVec n → BitVec n → Bool) (g : BitVec n → BitVec n → BitVec n)
+    (a b : BitVec n) : iN n :=
 
-/- @OfNat.ofNat PNat 32  -/
+  if isPoison a b then poison else bitvec (g a b)
 
-/- BitVec.ofNat (↑32) 2 : BitVec ↑32 -/
+/--
+Equality between two `iN` values, returning an `iN 1` (boolean) result.
+
+LangRef: https://llvm.org/docs/LangRef.html#icmp-instruction
+-/
+@[iN_unwrap_inst]
+protected def iN.icmpEq {n} : iN n → iN n → iN 1 :=
+  iN.poisonWrapper (· == ·)
+
+/--
+LangRef: https://llvm.org/docs/LangRef.html#icmp-instruction
+-/
+@[iN_unwrap_inst]
+protected def iN.icmpNe {n} : iN n → iN n → iN 1 :=
+  iN.poisonWrapper (fun x1 x2 => decide (x1 != x2))
+
+/--
+LangRef: https://llvm.org/docs/LangRef.html#icmp-instruction
+-/
+@[iN_unwrap_inst]
+protected def iN.icmpUlt {n} : iN n → iN n → iN 1 :=
+  iN.poisonWrapper (fun x1 x2 => decide (x1.toNat < x2.toNat))
+
+/--
+LangRef: https://llvm.org/docs/LangRef.html#icmp-instruction
+-/
+@[iN_unwrap_inst]
+protected def iN.icmpUle {n} : iN n → iN n → iN 1 :=
+  iN.poisonWrapper (fun x1 x2 => decide (x1 ≤ x2))
+
+/--
+LangRef: https://llvm.org/docs/LangRef.html#icmp-instruction
+-/
+@[iN_unwrap_inst]
+protected def iN.icmpUgt {n} : iN n → iN n → iN 1 :=
+  iN.poisonWrapper (fun x1 x2 => decide (x1 > x2))
+
+/--
+LangRef: https://llvm.org/docs/LangRef.html#icmp-instruction
+-/
+@[iN_unwrap_inst]
+protected def iN.icmpUge {n} : iN n → iN n → iN 1 :=
+  iN.poisonWrapper (fun x1 x2 => decide (x1 ≥ x2))
+
+/--
+LangRef: https://llvm.org/docs/LangRef.html#icmp-instruction
+-/
+@[iN_unwrap_inst]
+protected def iN.icmpSlt {n} : iN n → iN n → iN 1 :=
+  iN.poisonWrapper (fun x1 x2 => x1.slt x2)
+
+/--
+LangRef: https://llvm.org/docs/LangRef.html#icmp-instruction
+-/
+@[iN_unwrap_inst]
+protected def iN.icmpSle {n} : iN n → iN n → iN 1 :=
+  iN.poisonWrapper (fun x1 x2 => x1.sle x2)
+
+/--
+LangRef: https://llvm.org/docs/LangRef.html#icmp-instruction
+-/
+@[iN_unwrap_inst]
+protected def iN.icmpSgt {n} : iN n → iN n → iN 1 :=
+  iN.poisonWrapper (fun x1 x2 => !x1.sle x2)
+
+/--
+LangRef: https://llvm.org/docs/LangRef.html#icmp-instruction
+-/
+@[iN_unwrap_inst]
+protected def iN.icmpSge {n} : iN n → iN n → iN 1 :=
+  iN.poisonWrapper (fun x1 x2 => !x1.slt x2)
+
+@[inherit_doc] infixl:55 " ==ᵤ " => iN.icmpEq
+@[inherit_doc] infixl:55 " !=ᵤ " => iN.icmpNe
+@[inherit_doc] infixl:55 " <ᵤ "  => iN.icmpUlt
+@[inherit_doc] infixl:55 " ≤ᵤ "  => iN.icmpUle
+@[inherit_doc] infixl:55 " >ᵤ "  => iN.icmpUgt
+@[inherit_doc] infixl:55 " ≥ᵤ "  => iN.icmpUge
+@[inherit_doc] infixl:55 " <ₛ "  => iN.icmpSlt
+@[inherit_doc] infixl:55 " ≤ₛ "  => iN.icmpSle
+@[inherit_doc] infixl:55 " >ₛ "  => iN.icmpSgt
+@[inherit_doc] infixl:55 " ≥ₛ "  => iN.icmpSge
+
+/--
+LangRef: https://llvm.org/docs/LangRef.html#and-instruction
+-/
+@[iN_unwrap_inst]
+protected def iN.and {n} : iN n → iN n → iN n :=
+  iN.poisonWrapper (· &&& ·)
+
+/--
+LangRef: https://llvm.org/docs/LangRef.html#or-instruction
+-/
+@[iN_unwrap_inst]
+protected def iN.or {n} : iN n → iN n → iN n :=
+  iN.poisonWrapper (· ||| ·)
+
+instance {n} : HAnd (iN n) (iN n) (iN n) where
+  hAnd := iN.and
+
+instance {n} : HOr (iN n) (iN n) (iN n) where
+  hOr := iN.or
+
+@[iN_unwrap_inst]
+protected def iN.addBV {n : Nat} (a b : BitVec n) : iN n :=
+  bitvec (a + b)
 
 /--
 The integer sum of both operands. If the sum overflows, the result is returned modulo 2ⁿ.
 
 LangRef: https://llvm.org/docs/LangRef.html#add-instruction
 -/
-@[iN_to_bitvec, iN_unwrap_poison]
-protected def iN.add {n} : iN n → iN n → iN n
-  | poison, _ => poison
-  | _, poison => poison
-  | bitvec a, bitvec b => bitvec (a + b)
+@[iN_unwrap_inst]
+protected def iN.add {n} : iN n → iN n → iN n :=
+  iN.poisonWrapper iN.addBV
 
-@[iN_to_bitvec]
+@[iN_unwrap_inst]
 protected def iN.addNswBV {n : Nat} (a b : BitVec n) : iN n :=
-  if BitVec.saddOverflow a b then
-    poison
-  else
-    bitvec (a + b)
+  iN.poisonPreconditions BitVec.saddOverflow (· + ·) a b
 
 /--
 The integer sum of both operands. If the signed sum overflows, poison is returned.
 
 LangRef: https://llvm.org/docs/LangRef.html#add-instruction
 -/
-@[iN_unwrap_poison, iN_to_bitvec]
-protected def iN.addNsw {n} : iN n → iN n → iN n
-  | poison, _ => poison
-  | _, poison => poison
-  | bitvec a, bitvec b => iN.addNswBV a b
+@[iN_unwrap_inst]
+protected def iN.addNsw {n} : iN n → iN n → iN n :=
+  iN.poisonWrapper iN.addNswBV
 
-@[iN_to_bitvec]
+@[iN_unwrap_inst]
 protected def iN.addNuwBV {n : Nat} (a b : BitVec n) : iN n :=
-  if BitVec.uaddOverflow a b then
-    poison
-  else
-    bitvec (a + b)
+  iN.poisonPreconditions BitVec.uaddOverflow (· + ·) a b
 
 /--
 The integer sum of both operands. If the unsigned sum overflows, poison is returned.
 
 LangRef: https://llvm.org/docs/LangRef.html#add-instruction
 -/
-@[iN_unwrap_poison, iN_to_bitvec]
-protected def iN.addNuw {n} : iN n → iN n → iN n
-  | poison, _ => poison
-  | _, poison => poison
-  | bitvec a, bitvec b => iN.addNuwBV a b
+@[iN_unwrap_inst]
+protected def iN.addNuw {n} : iN n → iN n → iN n :=
+  iN.poisonWrapper iN.addNuwBV
 
-@[iN_to_bitvec]
+@[iN_unwrap_inst]
 protected def iN.addNwBV {n : Nat} (a b : BitVec n) : iN n :=
-  if BitVec.saddOverflow a b || BitVec.uaddOverflow a b then
-    poison
-  else
-    bitvec (a + b)
+  let isPoison := fun x y => BitVec.saddOverflow x y || BitVec.uaddOverflow x y
+  iN.poisonPreconditions isPoison (· + ·) a b
 
 /--
 The integer sum of both operands. If the sum overflows, poison is returned. Equivalent to `add nsw nuw`.
 
 LangRef: https://llvm.org/docs/LangRef.html#add-instruction
 -/
-@[iN_unwrap_poison, iN_to_bitvec]
-protected def iN.addNw {n} : iN n → iN n → iN n
-  | poison, _ => poison
-  | _, poison => poison
-  | bitvec a, bitvec b => iN.addNwBV a b
+@[iN_unwrap_inst]
+protected def iN.addNw {n} : iN n → iN n → iN n :=
+  iN.poisonWrapper iN.addNwBV
 
 instance : Add (iN n) where
   add := iN.add
-
---attribute [iN_unwrap_poison, iN_to_bitvec] iN.add
-
-@[iN_to_bitvec, iN_unwrap_poison]
-private theorem iN.add_rewrite_proper {n} {x y : iN n} :
-  x + y = iN.add x y := rfl
 
 @[inherit_doc] infixl:65 " +nsw " => iN.addNsw
 @[inherit_doc] infixl:65 " +nuw " => iN.addNuw
 @[inherit_doc] infixl:65 " +nw "  => iN.addNw
 
-/--
+/- /--
 The integer difference of both operands. If the difference overflows, the result is returned modulo 2ⁿ.
 
 LangRef: https://llvm.org/docs/LangRef.html#sub-instruction
 -/
-@[iN_to_bitvec]
+@[iN_unwrap_inst]
 protected def iN.sub {n} : iN n → iN n → iN n
   | poison, _ => poison
   | _, poison => poison
   | bitvec a, bitvec b => bitvec (a - b)
 
-@[iN_to_bitvec]
+@[iN_unwrap_inst]
 protected def iN.subNswBV {n : Nat} (a b : BitVec n) : iN n :=
   if BitVec.ssubOverflow a b then
     poison
@@ -146,13 +229,13 @@ The integer difference of both operands. If the signed difference overflows, poi
 
 LangRef: https://llvm.org/docs/LangRef.html#sub-instruction
 -/
-@[iN_unwrap_poison, iN_to_bitvec]
+@[iN_unwrap_inst]
 protected def iN.subNsw {n} : iN n → iN n → iN n
   | poison, _ => poison
   | _, poison => poison
   | bitvec a, bitvec b => iN.subNswBV a b
 
-@[iN_to_bitvec]
+@[iN_unwrap_inst]
 protected def iN.subNuwBV {n : Nat} (a b : BitVec n) : iN n :=
   if BitVec.usubOverflow a b then
     poison
@@ -164,13 +247,13 @@ The integer difference of both operands. If the unsigned difference overflows, p
 
 LangRef: https://llvm.org/docs/LangRef.html#sub-instruction
 -/
-@[iN_unwrap_poison, iN_to_bitvec]
+@[iN_unwrap_inst]
 protected def iN.subNuw {n} : iN n → iN n → iN n
   | poison, _ => poison
   | _, poison => poison
   | bitvec a, bitvec b => iN.subNuwBV a b
 
-@[iN_to_bitvec]
+@[iN_unwrap_inst]
 protected def iN.subNwBV {n : Nat} (a b : BitVec n) : iN n :=
   if BitVec.ssubOverflow a b || BitVec.usubOverflow a b then
     poison
@@ -182,7 +265,7 @@ The integer difference of both operands. If the difference overflows, poison is 
 
 LangRef: https://llvm.org/docs/LangRef.html#sub-instruction
 -/
-@[iN_unwrap_poison, iN_to_bitvec]
+@[iN_unwrap_inst]
 protected def iN.subNw {n} : iN n → iN n → iN n
   | poison, _ => poison
   | _, poison => poison
@@ -193,15 +276,15 @@ instance : Sub (iN n) where
 
 @[inherit_doc] infixl:65 " -nsw " => iN.subNsw
 @[inherit_doc] infixl:65 " -nuw " => iN.subNuw
-@[inherit_doc] infixl:65 " -nw "  => iN.subNw
+@[inherit_doc] infixl:65 " -nw "  => iN.subNw -/
 
-/- @[iN_to_bitvec]
+/- @[iN_unwrap_inst]
 protected def iN.sub {n} : iN n → iN n → iN n
   | poison, _ => poison
   | _, poison => poison
   | bitvec a, bitvec b => a - b
 
-@[iN_to_bitvec]
+@[iN_unwrap_inst]
 protected def iN.sub_nsw {n} : iN n → iN n → iN n
   | poison, _ => poison
   | _, poison => poison
@@ -211,7 +294,7 @@ protected def iN.sub_nsw {n} : iN n → iN n → iN n
     else
       a - b
 
-@[iN_to_bitvec]
+@[iN_unwrap_inst]
 protected def iN.sub_nuw {n} : iN n → iN n → iN n
   | poison, _ => poison
   | _, poison => poison
@@ -221,13 +304,13 @@ protected def iN.sub_nuw {n} : iN n → iN n → iN n
     else
       a - b -/
 
-/- @[iN_to_bitvec]
+/- @[iN_unwrap_inst]
 protected def iN.mul {n} : iN n → iN n → iN n
   | poison, _ => poison
   | _, poison => poison
   | bitvec a, bitvec b => a * b
 
-@[iN_to_bitvec]
+@[iN_unwrap_inst]
 protected def iN.mul_nsw {n} : iN n → iN n → iN n
   | poison, _ => poison
   | _, poison => poison
@@ -237,7 +320,7 @@ protected def iN.mul_nsw {n} : iN n → iN n → iN n
     else
       a * b
 
-@[iN_to_bitvec]
+@[iN_unwrap_inst]
 protected def iN.mul_nuw {n} : iN n → iN n → iN n
   | poison, _ => poison
   | _, poison => poison
@@ -247,7 +330,7 @@ protected def iN.mul_nuw {n} : iN n → iN n → iN n
     else
       a * b
 
-@[iN_to_bitvec]
+@[iN_unwrap_inst]
 protected def iN.mul_nw {n} : iN n → iN n → iN n
   | poison, _ => poison
   | _, poison => poison
@@ -257,7 +340,7 @@ protected def iN.mul_nw {n} : iN n → iN n → iN n
     else
       a * b
 
-@[iN_to_bitvec]
+@[iN_unwrap_inst]
 protected def iN.udiv {n} : iN n → iN n → iN n
   | poison, _ => poison
   | _, poison => poison
@@ -269,7 +352,7 @@ protected def iN.udiv {n} : iN n → iN n → iN n
     else
       a / b
 
-@[iN_to_bitvec]
+@[iN_unwrap_inst]
 protected def iN.sdiv {n} {z : n != 0} : iN n → iN n → iN n
   | poison, _ => poison
   | _, poison => poison
@@ -281,7 +364,7 @@ protected def iN.sdiv {n} {z : n != 0} : iN n → iN n → iN n
       a.sdiv b
 
 /-- Division by `0` in `iN 0` is defined to be `0`, not poison.  -/
-@[iN_to_bitvec]
+@[iN_unwrap_inst]
 protected def iN.udiv_exact {n} : iN n → iN n → iN n
   | poison, _ => poison
   | _, poison => poison
@@ -294,7 +377,7 @@ protected def iN.udiv_exact {n} : iN n → iN n → iN n
       a / b
 
 /-- Division by `0` in `iN 0` is defined to be `0`, not poison.  -/
-@[iN_to_bitvec]
+@[iN_unwrap_inst]
 protected def iN.sdiv_exact {n} : iN n → iN n → iN n
   | poison, _ => poison
   | _, poison => poison
@@ -307,7 +390,7 @@ protected def iN.sdiv_exact {n} : iN n → iN n → iN n
       a.sdiv b
 
 /-- Division by `0` in `iN 0` is defined to be `0`, not poison.  -/
-@[iN_to_bitvec]
+@[iN_unwrap_inst]
 protected def iN.urem {n} : iN n → iN n → iN n
   | poison, _ => poison
   | _, poison => poison
@@ -320,7 +403,7 @@ protected def iN.urem {n} : iN n → iN n → iN n
       a % b
 
 /-- Division by `0` in `iN 0` is defined to be `0`, not poison.  -/
-@[iN_to_bitvec]
+@[iN_unwrap_inst]
 protected def iN.srem {n} : iN n → iN n → iN n
   | poison, _ => poison
   | _, poison => poison
@@ -332,25 +415,25 @@ protected def iN.srem {n} : iN n → iN n → iN n
     else
       a.srem b
 
-@[iN_to_bitvec]
+@[iN_unwrap_inst]
 protected def iN.and {n} : iN n → iN n → iN n
   | poison, _ => poison
   | _, poison => poison
   | bitvec a, bitvec b => a &&& b
 
-@[iN_to_bitvec]
+@[iN_unwrap_inst]
 protected def iN.or {n} : iN n → iN n → iN n
   | poison, _ => poison
   | _, poison => poison
   | bitvec a, bitvec b => a ||| b
 
-@[iN_to_bitvec]
+@[iN_unwrap_inst]
 protected def iN.xor {n} : iN n → iN n → iN n
   | poison, _ => poison
   | _, poison => poison
   | bitvec a, bitvec b => a ^^^ b
 
-@[iN_to_bitvec]
+@[iN_unwrap_inst]
 protected def iN.shl {n} : iN n → iN n → iN n
   | poison, _ => poison
   | _, poison => poison
@@ -364,7 +447,7 @@ protected def iN.shl {n} : iN n → iN n → iN n
       a <<< s
 -/
 
-@[iN_to_bitvec]
+/- @[iN_unwrap_inst]
 protected def iN.shlNswClean {n : Nat} (a : BitVec n) (b : BitVec n) : iN n :=
   let s := b.toNat
 
@@ -378,32 +461,58 @@ protected def iN.shlNswClean {n : Nat} (a : BitVec n) (b : BitVec n) : iN n :=
     else
       bitvec res
 
-@[iN_unwrap_poison, iN_to_bitvec]
+@[iN_unwrap_inst]
 protected def iN.shlNsw {n} : iN n → iN n → iN n
   | poison, _ => poison
   | _, poison => poison
-  | bitvec a, bitvec b => iN.shlNswClean a b
+  | bitvec a, bitvec b => iN.shlNswClean a b -/
 
 section norm_eqs
 /-! These simp-lemmas rewrite the iN operations into equivalent notation -/
-@[simp, grind =] theorem add_eq (x y : iN n) : iN.add x y = x + y := rfl
-@[simp, grind =] theorem addNsw_eq (x y : iN n) : iN.addNsw x y = x +nsw y := rfl
-@[simp, grind =] theorem addNuw_eq (x y : iN n) : iN.addNuw x y = x +nuw y := rfl
-@[simp, grind =] theorem addNw_eq (x y : iN n) : iN.addNw x y = x +nw y := rfl
-@[simp, grind =] theorem sub_eq (x y : iN n) : iN.sub x y = x - y := rfl
+@[grind =] theorem icmpEq_eq (x y : iN n) : iN.icmpEq x y = (x ==ᵤ y) := rfl
+@[grind =] theorem icmpNe_eq (x y : iN n) : iN.icmpNe x y = (x !=ᵤ y) := rfl
+@[grind =] theorem icmpUlt_eq (x y : iN n) : iN.icmpUlt x y = (x <ᵤ y) := rfl
+@[grind =] theorem icmpUle_eq (x y : iN n) : iN.icmpUle x y = (x ≤ᵤ y) := rfl
+@[grind =] theorem icmpUgt_eq (x y : iN n) : iN.icmpUgt x y = (x >ᵤ y) := rfl
+@[grind =] theorem icmpUge_eq (x y : iN n) : iN.icmpUge x y = (x ≥ᵤ y) := rfl
+@[grind =] theorem icmpSlt_eq (x y : iN n) : iN.icmpSlt x y = (x <ₛ y) := rfl
+@[grind =] theorem icmpSle_eq (x y : iN n) : iN.icmpSle x y = (x ≤ₛ y) := rfl
+@[grind =] theorem icmpSgt_eq (x y : iN n) : iN.icmpSgt x y = (x >ₛ y) := rfl
+@[grind =] theorem icmpSge_eq (x y : iN n) : iN.icmpSge x y = (x ≥ₛ y) := rfl
+@[grind =] theorem and_eq (x y : iN n) : iN.and x y = x &&& y := rfl
+@[grind =] theorem or_eq (x y : iN n) : iN.or x y = x ||| y := rfl
+@[grind =] theorem add_eq (x y : iN n) : iN.add x y = x + y := rfl
+@[grind =] theorem addNsw_eq (x y : iN n) : iN.addNsw x y = x +nsw y := rfl
+@[grind =] theorem addNuw_eq (x y : iN n) : iN.addNuw x y = x +nuw y := rfl
+@[grind =] theorem addNw_eq (x y : iN n) : iN.addNw x y = x +nw y := rfl
+/- @[simp, grind =] theorem sub_eq (x y : iN n) : iN.sub x y = x - y := rfl
 @[simp, grind =] theorem subNsw_eq (x y : iN n) : iN.subNsw x y = x -nsw y := rfl
 @[simp, grind =] theorem subNuw_eq (x y : iN n) : iN.subNuw x y = x -nuw y := rfl
-@[simp, grind =] theorem subNw_eq (x y : iN n) : iN.subNw x y = x -nw y := rfl
+@[simp, grind =] theorem subNw_eq (x y : iN n) : iN.subNw x y = x -nw y := rfl -/
 end norm_eqs
 
+@[iN_unwrap_inst, grind =] theorem bitvec_addNsw_eq_thing (x y : BitVec n) : (bitvec x) +nsw (bitvec y) = iN.addNswBV x y := rfl
+
 section norm_eqs_to_bitvec
-/-! When using iN_to_bitvec, these simp-lemmas rewrite the notation into back into iN, so they can be lowered -/
-@[iN_to_bitvec, grind =] theorem bitvec_add_eq (x y : iN n) : x + y = iN.add x y := rfl
-@[iN_to_bitvec, grind =] theorem bitvec_addNsw_eq (x y : iN n) : x +nsw y = iN.addNsw x y := rfl
-@[iN_to_bitvec, grind =] theorem bitvec_addNuw_eq (x y : iN n) : x +nuw y = iN.addNuw x y := rfl
-@[iN_to_bitvec, grind =] theorem bitvec_addNw_eq (x y : iN n) : x +nw y = iN.addNw x y := rfl
-@[iN_to_bitvec, grind =] theorem bitvec_sub_eq (x y : iN n) : x - y = iN.sub x y := rfl
-@[iN_to_bitvec, grind =] theorem bitvec_subNsw_eq (x y : iN n) : x -nsw y = iN.subNsw x y := rfl
-@[iN_to_bitvec, grind =] theorem bitvec_subNuw_eq (x y : iN n) : x -nuw y = iN.subNuw x y := rfl
-@[iN_to_bitvec, grind =] theorem bitvec_subNw_eq (x y : iN n) : x -nw y = iN.subNw x y := rfl
+/-! When using iN_unwrap_inst, these simp-lemmas rewrite the notation into back into iN, so they can be lowered -/
+@[iN_unwrap_inst, grind =] theorem bitvec_icmpEq_eq (x y : iN n) : (x ==ᵤ y) = iN.icmpEq x y := rfl
+@[iN_unwrap_inst, grind =] theorem bitvec_icmpNe_eq (x y : iN n) : (x !=ᵤ y) = iN.icmpNe x y := rfl
+@[iN_unwrap_inst, grind =] theorem bitvec_icmpUlt_eq (x y : iN n) : (x <ᵤ y) = iN.icmpUlt x y := rfl
+@[iN_unwrap_inst, grind =] theorem bitvec_icmpUle_eq (x y : iN n) : (x ≤ᵤ y) = iN.icmpUle x y := rfl
+@[iN_unwrap_inst, grind =] theorem bitvec_icmpUgt_eq (x y : iN n) : (x >ᵤ y) = iN.icmpUgt x y := rfl
+@[iN_unwrap_inst, grind =] theorem bitvec_icmpUge_eq (x y : iN n) : (x ≥ᵤ y) = iN.icmpUge x y := rfl
+@[iN_unwrap_inst, grind =] theorem bitvec_icmpSlt_eq (x y : iN n) : (x <ₛ y) = iN.icmpSlt x y := rfl
+@[iN_unwrap_inst, grind =] theorem bitvec_icmpSle_eq (x y : iN n) : (x ≤ₛ y) = iN.icmpSle x y := rfl
+@[iN_unwrap_inst, grind =] theorem bitvec_icmpSgt_eq (x y : iN n) : (x >ₛ y) = iN.icmpSgt x y := rfl
+@[iN_unwrap_inst, grind =] theorem bitvec_icmpSge_eq (x y : iN n) : (x ≥ₛ y) = iN.icmpSge x y := rfl
+@[iN_unwrap_inst, grind =] theorem bitvec_and_eq (x y : iN n) : x &&& y = iN.and x y := rfl
+@[iN_unwrap_inst, grind =] theorem bitvec_or_eq (x y : iN n) : x ||| y = iN.or x y := rfl
+@[iN_unwrap_inst, grind =] theorem bitvec_add_eq (x y : iN n) : x + y = iN.add x y := rfl
+@[iN_unwrap_inst, grind =] theorem bitvec_addNsw_eq (x y : iN n) : x +nsw y = iN.addNsw x y := rfl
+@[iN_unwrap_inst, grind =] theorem bitvec_addNuw_eq (x y : iN n) : x +nuw y = iN.addNuw x y := rfl
+@[iN_unwrap_inst, grind =] theorem bitvec_addNw_eq (x y : iN n) : x +nw y = iN.addNw x y := rfl
+/- @[iN_unwrap_inst, grind =] theorem bitvec_sub_eq (x y : iN n) : x - y = iN.sub x y := rfl
+@[iN_unwrap_inst, grind =] theorem bitvec_subNsw_eq (x y : iN n) : x -nsw y = iN.subNsw x y := rfl
+@[iN_unwrap_inst, grind =] theorem bitvec_subNuw_eq (x y : iN n) : x -nuw y = iN.subNuw x y := rfl
+@[iN_unwrap_inst, grind =] theorem bitvec_subNw_eq (x y : iN n) : x -nw y = iN.subNw x y := rfl -/
 end norm_eqs_to_bitvec
