theorems/iN/iN_lemmas.lean
@@ -4,6 +4,15 @@ import theorems.iN.iN_tactics
 import theorems.iN.iN_rewrite
 import theorems.Core.Attrs.Attrs
 
+/-- The supported bit sizes. Proofs do not need to prove ∀n : Nat. -/
+inductive Bits : Nat → Prop where
+  | i1 : Bits 1
+  | i8 : Bits 8
+  | i16 : Bits 16
+  | i32 : Bits 32
+  | i64 : Bits 64
+  | i128 : Bits 128
+
 @[grind =]
 theorem BitVec.saddOverflow_comm {n} (a b : BitVec n)
     : a.saddOverflow b = b.saddOverflow a := by
@@ -20,13 +29,158 @@ theorem BitVec.uaddOverflow_comm {n} (a b : BitVec n)
   unfold BitVec.uaddOverflow
   grind
 
+theorem BitVec.saddOverflow_chain_assoc_monotone {n} {hn : Bits n} (a b c : BitVec n)
+    (h : a.msb = b.msb ∧ b.msb = c.msb)
+
+    : (a.saddOverflow b || (a + b).saddOverflow c) =
+      (b.saddOverflow c || a.saddOverflow (b + c)) := by
+
+  cases hn
+  case i1   => bv_check "../../lrat/BitVec.saddOverflow_assoc_monotone-45-15.lrat"
+  case i8   => bv_check "../../lrat/BitVec.saddOverflow_assoc_monotone-46-15.lrat"
+  case i16  => bv_check "../../lrat/BitVec.saddOverflow_assoc_monotone-47-15.lrat"
+  case i32  => bv_check "../../lrat/BitVec.saddOverflow_assoc_monotone-48-15.lrat"
+  case i64  => bv_check "../../lrat/BitVec.saddOverflow_assoc_monotone-49-15.lrat"
+  case i128 => bv_check "../../lrat/BitVec.saddOverflow_assoc_monotone-50-15.lrat"
+
+/- theorem test : ∃ (n : Nat) (a b c : BitVec n),
+    ¬((a.saddOverflow b || (a + b).saddOverflow c) ==
+      (b.saddOverflow c || a.saddOverflow (b + c))) := by
+
+  exists 8, 127#8, 1#8, -1#8 -/
+
+theorem BitVec.uaddOverflow_chain_assoc {n} {hn : Bits n} (a b c : BitVec n)
+    : (a.uaddOverflow b || (a + b).uaddOverflow c) =
+      (b.uaddOverflow c || a.uaddOverflow (b + c)) := by
+
+  cases hn
+  case i1   => bv_check "../../lrat/iN_lemmas.lean-BitVec.uaddOverflow_chain_assoc-57-15.lrat"
+  case i8   => bv_check "../../lrat/iN_lemmas.lean-BitVec.uaddOverflow_chain_assoc-58-15.lrat"
+  case i16  => bv_check "../../lrat/iN_lemmas.lean-BitVec.uaddOverflow_chain_assoc-59-15.lrat"
+  case i32  => bv_check "../../lrat/iN_lemmas.lean-BitVec.uaddOverflow_chain_assoc-60-15.lrat"
+  case i64  => bv_check "../../lrat/iN_lemmas.lean-BitVec.uaddOverflow_chain_assoc-61-15.lrat"
+  case i128 => bv_check "../../lrat/iN_lemmas.lean-BitVec.uaddOverflow_chain_assoc-62-16.lrat"
+
 namespace iN
 
-@[grind =]
+@[simp, grind =]
+theorem eq_bitvec_inj {n} {a b : BitVec n} :
+    ((bitvec a : iN n) = (bitvec b : iN n)) ↔ a = b := by
+
+  constructor
+  · intro h
+    injection h
+  . intro h
+    rw [h]
+
+@[simp]
+theorem poisonWrapper_poison_left {n} {k} {g : BitVec n → BitVec n → iN k} {b : iN n} :
+  iN.poisonWrapper g poison b = poison := by simp [iN.poisonWrapper]
+
+@[simp]
+theorem poisonWrapper_poison_right {n} {k} {g : BitVec n → BitVec n → iN k} {a : iN n} :
+  iN.poisonWrapper g a poison = poison := by cases a <;> rfl
+
+@[simp]
+theorem poisonWrapper_bitvec_left {n} {k} {g : BitVec n → BitVec n → iN k} {a : BitVec n} {b : iN n} :
+  iN.poisonWrapper g (bitvec a) b = match b with
+    | poison => poison
+    | bitvec b' => g a b' := by cases b <;> rfl
+
+@[simp]
+theorem poisonWrapper_bitvec_right {n} {k} {g : BitVec n → BitVec n → iN k} {a : iN n} {b : BitVec n} :
+  iN.poisonWrapper g a (bitvec b) = match a with
+    | poison => poison
+    | bitvec a' => g a' b := by cases a <;> rfl
+
+@[simp]
+theorem poisonWrapper_bitvec {n} {k} {g : BitVec n → BitVec n → iN k} {a b : BitVec n} :
+  iN.poisonWrapper g (bitvec a) (bitvec b) = g a b := by cases a <;> rfl
+
+/-- Simplifying lemma about poisonable equations of the form `(a ⋄₁ b) ⋄₂ c`. -/
+@[simp]
+theorem poisonPreconditions_match_wrapper_assoc_left {n}
+    (isPoison₁ : BitVec n → BitVec n → Bool)
+    (isPoison₂ : BitVec n → BitVec n → Bool)
+    (a b c : BitVec n)
+    (op₁ : BitVec n → BitVec n → BitVec n)
+    (op₂ : BitVec n → BitVec n → BitVec n)
+    : (match iN.poisonPreconditions isPoison₁ op₁ a b with
+      | poison => poison
+      | bitvec ab' => iN.poisonPreconditions isPoison₂ op₂ ab' c)
+
+      = bif isPoison₁ a b || isPoison₂ (op₁ a b) c then
+        poison
+      else
+        bitvec (op₂ (op₁ a b) c) := by
+
+  unfold iN.poisonPreconditions
+  cases isPoison₁ a b
+  . simp
+  . simp
+
+/-- Simplifying lemma about poisonable equations of the form `a ⋄₁ (b ⋄₂ c)`. -/
+@[simp]
+theorem poisonPreconditions_match_wrapper_assoc_right {n}
+    (isPoison₁ : BitVec n → BitVec n → Bool)
+    (isPoison₂ : BitVec n → BitVec n → Bool)
+    (a b c : BitVec n)
+    (op₁ : BitVec n → BitVec n → BitVec n)
+    (op₂ : BitVec n → BitVec n → BitVec n)
+    : (match iN.poisonPreconditions isPoison₂ op₂ b c with
+      | poison => poison
+      | bitvec bc' => iN.poisonPreconditions isPoison₁ op₁ a bc')
+
+      = bif isPoison₂ b c || isPoison₁ a (op₂ b c) then
+        poison
+      else
+        bitvec (op₁ a (op₂ b c)) := by
+
+  unfold iN.poisonPreconditions
+  cases isPoison₂ b c
+  . simp
+  . simp
+
+@[simp]
+theorem bitvec_cond {n} (c : Bool) (t e : BitVec n) :
+    cond c (bitvec t) (bitvec e) = bitvec (cond c t e) := by
+  cases c <;> rfl
+
+/-- Forces unfolds when about to be simplified -/
+@[simp]
+theorem poisonPreconditions_rewrite_unfold {n} (a b : BitVec n) (c : iN n)
+    (isPoison : BitVec n → BitVec n → Bool) (op : BitVec n → BitVec n → BitVec n)
+    : (iN.poisonPreconditions isPoison op a b ~> c) =
+      ((if isPoison a b then poison else bitvec (op a b)) ~> c) := by
+
+  unfold iN.poisonPreconditions
+  rfl
+
+/-- Forces unfolds when about to be simplified -/
+@[simp]
+theorem poisonPreconditions_rewrite_iff_unfold_left {n} (a b : BitVec n) (c : iN n)
+    (isPoison : BitVec n → BitVec n → Bool) (op : BitVec n → BitVec n → BitVec n)
+    : (iN.poisonPreconditions isPoison op a b <~> c) =
+      ((if isPoison a b then poison else bitvec (op a b)) <~> c) := by
+
+  unfold iN.poisonPreconditions
+  rfl
+
+/-- Forces unfolds when about to be simplified -/
+@[simp]
+theorem poisonPreconditions_rewrite_iff_unfold_right {n} (a b : BitVec n) (c : iN n)
+    (isPoison : BitVec n → BitVec n → Bool) (op : BitVec n → BitVec n → BitVec n)
+    : (c <~> iN.poisonPreconditions isPoison op a b) =
+      (c <~> (if isPoison a b then poison else bitvec (op a b))) := by
+
+  unfold iN.poisonPreconditions
+  rfl
+
+/- @[grind =]
 theorem addNswBV_comm {n} {a b : BitVec n}
     : iN.addNswBV a b = iN.addNswBV b a := by
 
-  simp [iN_to_bitvec]
+  simp only [iN_to_bitvec]
   rw [BitVec.saddOverflow_comm]
   split <;> try simp
 
@@ -38,13 +192,13 @@ theorem addNswBV_comm {n} {a b : BitVec n}
 theorem addNuwBV_comm {n} {a b : BitVec n}
     : iN.addNuwBV a b = iN.addNuwBV b a := by
 
-  simp [iN_to_bitvec]
+  simp only [iN_to_bitvec]
   rw [BitVec.uaddOverflow_comm]
   split <;> try simp
 
   -- h✝ : ¬b.uaddOverflow a = true
   -- ⊢ a + b = b + a
-  grind
+  grind -/
 
 end iN
 
