theorems/iN_basic/add.lean
@@ -8,76 +8,118 @@ namespace iN
 theorem add_comm {n} (x y : iN n)
     : x + y = y + x := by
 
-  -- clear poison from `x` and `y`
-  simp only [iN_unwrap_poison]
-  repeat' split; <;> try simp [*] at *
-
-  grind
+  poison_unroll x y => a b
+  simp [iN_unwrap_inst]
+  rw [BitVec.add_comm a b]
 
 @[grind]
 theorem addNsw_comm {n} (x y : iN n)
     : x +nsw y <~> y +nsw x := by
 
-  -- clear poison from `x` and `y`
-  simp only [iN_unwrap_poison]
-
-  cases x
-  . cases y
-    . simp [*] at *
-      grind
-    . simp
-  . simp
-    -- TODO https://leanprover.zulipchat.com/#narrow/channel/113488-general/topic/Simp.20not.20collapsing.20simultaneous.20matching/with/538586043
-    grind
+  poison_unroll x y => a b
+  simp [iN_unwrap_inst]
+  rw [BitVec.saddOverflow_comm a b]
+  rw [BitVec.add_comm a b]
 
 @[grind]
 theorem addNuw_comm {n} (x y : iN n)
     : x +nuw y <~> y +nuw x := by
 
-  -- clear poison from `x` and `y`
-  simp only [iN_unwrap_poison]
+  poison_unroll x y => a b
+  simp [iN_unwrap_inst]
+  rw [BitVec.uaddOverflow_comm a b]
+  rw [BitVec.add_comm a b]
 
-  cases x
-  . cases y
-    . simp [*] at *
-      grind
-    . simp
-  . simp
-    -- TODO https://leanprover.zulipchat.com/#narrow/channel/113488-general/topic/Simp.20not.20collapsing.20simultaneous.20matching/with/538586043
-    grind
+@[grind]
+theorem addNw_comm {n} (x y : iN n)
+    : x +nw y <~> y +nw x := by
+
+  poison_unroll x y => a b
+  simp [iN_unwrap_inst]
+  rw [BitVec.add_comm a b]
+  rw [BitVec.saddOverflow_comm a b]
+  rw [BitVec.uaddOverflow_comm a b]
+
+@[grind]
+theorem addNsw_refine {n} (x y : iN n)
+  : x +nsw y ~> x + y := by
+
+  poison_unroll x y => a b
+
+  simp [iN_unwrap_inst]
+  if h : a.saddOverflow b then
+    simp [h]
+  else
+    simp [h]
+
+@[grind]
+theorem addNuw_refine {n} (x y : iN n)
+  : x +nuw y ~> x + y := by
+
+  poison_unroll x y => a b
+
+  simp [iN_unwrap_inst]
+  if h : a.uaddOverflow b then
+    simp [h]
+  else
+    simp [h]
+
+@[grind]
+theorem addNw_refine {n} (x y : iN n)
+  : x +nw y ~> x + y := by
+
+  poison_unroll x y => a b
+
+  simp [iN_unwrap_inst]
+  if h1 : (a.saddOverflow b ∨ a.uaddOverflow b) then
+    simp [h1]
+  else
+    simp [h1]
 
 @[grind]
 theorem add_assoc {n} (x y z : iN n)
     : (x + y) + z = x + (y + z) := by
 
-  -- clear poison from `x` and `y`
-  simp only [iN_unwrap_poison]
+  poison_unroll x y z => a b c
+  simp [iN_unwrap_inst]
+  rw [BitVec.add_assoc a b c]
 
-  cases x
-  . cases y
-    . cases z
-      . simp
-        grind
-      . simp
-    . simp
-  . simp
+@[grind]
+theorem addNsw_not_assoc : ∃ (n : Nat) (x y z : iN n),
+    ¬(x +nsw y) +nsw z <~> x +nsw (y +nsw z) := by
 
-/- @[grind]
-theorem addNsw_assoc {n} (x y z : iN n)
+  exists 4
+  exists 6, 5, bitvec (BitVec.neg 7)
+
+  simp [iN_unwrap_inst, BitVec.saddOverflow]
+
+@[grind]
+theorem addNsw_assoc_same_sign {n} {hn : Bits n} (x y z : iN n)
+    (h :
+      (x ≥ₛ 0) &&& (y ≥ₛ 0) &&& (z ≥ₛ 0) ~> 1 ∨
+      (x <ₛ 0) &&& (y <ₛ 0) &&& (z <ₛ 0) ~> 1)
+
     : (x +nsw y) +nsw z <~> x +nsw (y +nsw z) := by
 
-  -- clear poison from `x` and `y`
-  simp only [iN_unwrap_poison]
+  poison_unroll x y z => a b c
+  simp [iN_unwrap_inst] at *
 
-  cases x
-  . cases y
-    . cases z
-      . simp
+  have h' : a.msb = b.msb ∧ b.msb = c.msb := by
+    bv_decide
 
+  rw [BitVec.saddOverflow_chain_assoc_monotone a b c h']
+  rw [BitVec.add_assoc a b c]
+  exact hn
 
+@[grind]
+theorem addNuw_assoc {n} {hn : Bits n} (x y z : iN n)
+    : (x +nuw y) +nuw z <~> x +nuw (y +nuw z) := by
 
-      . simp
-    . simp
-  . simp -/
+  poison_unroll x y z => a b c
+
+  simp [iN_unwrap_inst]
+  rw [BitVec.uaddOverflow_chain_assoc a b c]
+  rw [BitVec.add_assoc a b c]
+  exact hn
 
 end iN
